fix beta.v

src/FcEtt/fc_wf.v
@@ -1,5 +1,3 @@
-Require Import FcEtt.sigs.
-
 Require Export FcEtt.imports.
 Require Export FcEtt.ett_inf.
 Require Export FcEtt.ett_ind.
@@ -17,20 +15,27 @@ Set Implicit Arguments.
 (* ---------------------------------------------------- *)
 
 Lemma ann_ctx_wff_mutual :
-  (forall G0 a A, AnnTyping G0 a A -> AnnCtx G0) /\
-  (forall G0 phi,   AnnPropWff G0 phi -> AnnCtx G0) /\
-  (forall G0 D g p1 p2, AnnIso G0 D g p1 p2 -> AnnCtx G0) /\
-  (forall G0 D g A B,   AnnDefEq G0 D g A B -> AnnCtx G0) /\
+  (forall G0 psi a A, AnnTyping G0 psi a A -> AnnCtx G0) /\
+  (forall G0 psi phi,   AnnPropWff G0 psi phi -> AnnCtx G0) /\
+  (forall G0 psi g p1 p2, AnnIso G0 psi g p1 p2 -> AnnCtx G0) /\
+  (forall G0 psi g A B,   AnnDefEq G0 psi g A B -> AnnCtx G0) /\
   (forall G0, AnnCtx G0 -> True).
 Proof.
   eapply ann_typing_wff_iso_defeq_mutual; eauto.
 Qed.
 
 
-Definition AnnTyping_AnnCtx  := first  ann_ctx_wff_mutual.
-Definition AnnPropWff_AnnCtx := second ann_ctx_wff_mutual.
-Definition AnnIso_AnnCtx     := third  ann_ctx_wff_mutual.
-Definition AnnDefEq_AnnCtx   := fourth ann_ctx_wff_mutual.
+Lemma AnnTyping_AnnCtx : forall G0 psi a A, AnnTyping G0 psi a A -> AnnCtx G0.
+Proof. sfirstorder use:ann_ctx_wff_mutual. Qed.
+
+Lemma AnnPropWff_AnnCtx : forall G0 psi phi,   AnnPropWff G0 psi phi -> AnnCtx G0.
+Proof. sfirstorder use:ann_ctx_wff_mutual. Qed.
+
+Lemma AnnIso_AnnCtx : forall G0 psi g p1 p2, AnnIso G0 psi g p1 p2 -> AnnCtx G0.
+Proof. sfirstorder use:ann_ctx_wff_mutual. Qed.
+
+Lemma AnnDefEq_AnnCtx : forall G0 psi g A B,   AnnDefEq G0 psi g A B -> AnnCtx G0.
+Proof. sfirstorder use:ann_ctx_wff_mutual. Qed.
 
 Hint Resolve AnnTyping_AnnCtx AnnPropWff_AnnCtx AnnIso_AnnCtx
      AnnDefEq_AnnCtx : ctx_wff.
@@ -63,28 +68,39 @@ Hint Resolve AnnCtx_uniq.
 Hint Resolve lc_open_switch_co : lc.
 
 Lemma lc_mutual :
-  (forall G0 a A, AnnTyping G0 a A -> lc_tm a /\ lc_tm A) /\
-  (forall G0 phi, AnnPropWff G0 phi -> lc_constraint phi) /\
-  (forall G0 D g p1 p2, AnnIso G0 D g p1 p2 -> lc_constraint p1 /\ lc_constraint p2 /\ lc_co g) /\
-  (forall G0 D g A B,  AnnDefEq G0 D g A B -> lc_tm A /\ lc_tm B /\ lc_co g) /\
-  (forall G0, AnnCtx G0 -> forall x s , binds x s G0 -> lc_sort s).
+  (forall G0 psi a A, AnnTyping G0 psi a A -> lc_tm a /\ lc_tm A) /\
+  (forall G0 psi phi, AnnPropWff G0 psi phi -> lc_constraint phi) /\
+  (forall G0 psi g p1 p2, AnnIso G0 psi g p1 p2 -> lc_constraint p1 /\ lc_constraint p2 /\ lc_co g) /\
+  (forall G0 psi g A B,  AnnDefEq G0 psi g A B -> lc_tm A /\ lc_tm B /\ lc_co g) /\
+  (forall G0, AnnCtx G0 -> forall x psi s , binds x (psi, s) G0 -> lc_sort s).
 Proof.
   apply ann_typing_wff_iso_defeq_mutual.
   all: pre; basic_solve_n 2; split_hyp.
   all: lc_solve.
 Qed.
 
-Definition AnnTyping_lc  := first lc_mutual.
-Definition AnnPropWff_lc := second lc_mutual.
-Definition AnnIso_lc     := third lc_mutual.
-Definition AnnDefEq_lc   := fourth lc_mutual.
-Definition AnnCtx_lc     := fifth lc_mutual.
 
-Lemma AnnTyping_lc1 : forall G a A, AnnTyping G a A -> lc_tm a.
+
+Lemma AnnTyping_lc : forall G0 psi a A, AnnTyping G0 psi a A -> lc_tm a /\ lc_tm A.
+Proof. sfirstorder use:ann_ctx_wff_mutual. Qed.
+
+Lemma AnnPropWff_lc : forall G0 psi phi, AnnPropWff G0 psi phi -> lc_constraint phi.
+Proof. sfirstorder use:ann_ctx_wff_mutual. Qed.
+
+Lemma AnnIso_lc : forall G0 psi g p1 p2, AnnIso G0 psi g p1 p2 -> lc_constraint p1 /\ lc_constraint p2 /\ lc_co g.
+Proof. sfirstorder use:ann_ctx_wff_mutual. Qed.
+
+Lemma AnnDefEq_lc : forall G0 psi g A B,  AnnDefEq G0 psi g A B -> lc_tm A /\ lc_tm B /\ lc_co g.
+Proof. sfirstorder use:ann_ctx_wff_mutual. Qed.
+
+Lemma AnnCtx_lc : forall G0, AnnCtx G0 -> forall x psi s , binds x (psi, s) G0 -> lc_sort s.
+Proof. sfirstorder use:ann_ctx_wff_mutual. Qed.
+
+Lemma AnnTyping_lc1 : forall G psi a A, AnnTyping G psi a A -> lc_tm a.
 Proof.
   intros G a A H. destruct (AnnTyping_lc H); auto.
 Qed.
-Lemma AnnTyping_lc2 : forall G a A, AnnTyping G a A -> lc_tm A.
+Lemma AnnTyping_lc2 : forall G psi a A, AnnTyping G psi a A -> lc_tm A.
   intros G a A H. destruct (AnnTyping_lc H); auto.
 Qed.
 
@@ -104,7 +120,7 @@ Proof. intros. destruct (AnnDefEq_lc H); split_hyp; auto. Qed.
 Hint Resolve AnnTyping_lc1 AnnTyping_lc2 AnnIso_lc1 AnnIso_lc2 AnnIso_lc3 AnnDefEq_lc1 AnnDefEq_lc2 AnnDefEq_lc3 AnnCtx_lc : lc.
 
 
-Lemma AnnToplevel_lc : forall c s, binds c s an_toplevel -> lc_sig_sort s.
+Lemma AnnToplevel_lc : forall c psi0 s, binds c (psi0, s) an_toplevel -> lc_sig_sort s.
 Proof. induction AnnSig_an_toplevel.
        intros; lc_solve.
        all: intros; lc_solve_binds; split_hyp; subst; eauto with lc.
